\documentclass[../main/main.tex]{subfiles}


\begin{document}

\section{April 22th, 2020}
\subsection{Continuation of the Heat Equation}
From last time, we had: \[
	\tan (L \sqrt{-V}) = -\frac{k_0}{h}\sqrt{-C} = -\frac{\kappa_0}{hL}(L\sqrt{-C} ) 
.\] Thus if we let $L \sqrt{-C}  = z \implies C = - \left( \frac{z}{L} \right) ^2$, then we want to find the solutions to the equation: \[
\tan z = - \frac{\kappa_0}{hL}z
.\] With this, we would get: \[
\phi_n(x) = \sin(z_n \frac{x}{L})
.\] Since this is in the RSLP form, it has an associated dot product: \[
\phi_n\cdot \phi_m = \int^L_0 \phi_n(x) \phi_m(x) ~dx =  \begin{cases}
	0 , \quad p \neq q \\
	\frac{L}{2}\left( 1+\frac{\sin(2z_n)}{2z_n} \right) 
\end{cases}
.\] Note that the weight function $w(x) = 1$ (verify by comparing coefficients).

Going to the time equation: \[
	\beta_n'(t) - \gamma C_n \beta_n(t) = 0
.\] \[
\implies \beta_n'(t) + \gamma \left( \frac{z_n}{L} \right) ^2 \beta_n (t) = 0
.\] \[
\implies \beta_n(t) = e^{-\gamma\left( \frac{z_n}{L} \right) ^2 t}
.\] 

This gives us: \[
	v_n(x,t) = \phi_n(x) \beta_n(t) = e^{-\gamma\left( \frac{z_n}{L} \right) ^2 t} \sin \left( \frac{z_n}{L}x \right) 
.\] Meaning that the general solution is: \[
v(x,t) = \sum_{n=1}^{\infty} a_n e^{-\gamma\left( \frac{z)n}{L} \right) ^2t}\sin\left( \frac{z_n}{L}x \right) 
.\] For the initial condition, we have: \[
v(x,0) = \sum_{n=1}^{\infty} a_n \phi_n(x) = f(x) - u_e(x)
.\] \[
\implies a_n = \frac{ \phi_n\left( f-u_e \right) }{\phi_n\cdot \phi_n} =  \frac{1}{\frac{L}{2}\left( 1+ \frac{\sin(2z_n)}{2z_n} \right) }\int^L_0 (f(x) - u_e(x) ) \phi_n(x) ~dx, \quad n=1,2,3,..
.\] Thus the final solution is: \[
u(x,t) = u_e(x) + \sum_{n=1}^{\infty} a_n e^{-\gamma\left( \frac{z_n}{L} \right) ^2t}\phi_n(x)
.\] Note that the only difference between this solution and the wave equation is that the eigenvalues are different.

\begin{remark}
	Note that since $e^{-(\text{constant})t}$ approaches $0$ as $t$ increases, we have: \[
		\lim\limits_{t \to \infty} u(x,t) = u_e(x)
	.\] Note that this is not the case for the wave equation (unless there is a dampening term).
\end{remark}
\begin{remark}
	The wave equation with damping has the form: \[
	\frac{\partial ^2 u}{\partial x^2} = \frac{1}{v^2}\frac{\partial ^2 u}{\partial t^2} + b \frac{\partial u}{\partial t}  
.\] This will have a limiting solution equal to the time independent solution $u_e(x)$.
\end{remark}
\end{document}

